Pom/Lpo/Operations/Seq.lean
@@ -19,7 +19,7 @@ instance {α β : Lpofin (Label act test)} :
 
 def CopyFn_extends {α α' β β' : Lpofin (Label act test)}
     (hle : α ≤ α') (f : CopyFn α β) (g : CopyFn α' β') :=
-  ∀ φ : ↑α.branches, f φ ≤ g ⟨φ.val, branches_monotone hle φ.property⟩
+  ∀ φ : ↑α.branches, f φ ≤ g ⟨φ.val.up_cast hle, branches_monotone hle φ.property⟩
 
 open Classical in
 noncomputable def seq_base (α β : Lpofin (Label act test)) (f : CopyFn α β) :
@@ -29,24 +29,25 @@ noncomputable def seq_base (α β : Lpofin (Label act test)) (f : CopyFn α β) 
     α.rel x y ∨
     ∃ φ : ↑α.branches,
       (f φ).rel x y ∨
-      (φ ≤ α.form x ∧ y ∈ (f φ).nodes)
+      (φ.val.toForm ≤ α.form x ∧ y ∈ (f φ).nodes)
   lab x :=
     if hx : ∃ φ : ↑α.branches, x ∈ (f φ).nodes then
       (f hx.choose).lab x
     else
       α.lab x
-  form x :=
-    if x ∈ α.nodes then α.form x else Form.sOr fun φ : ↑α.branches ↦ ((f φ).form x).and φ.val
+  form x v :=
+    (α.form x v) ∨
+    (Form.sOr fun φ : ↑α.branches ↦ ((f φ).form x).and φ.val.toForm) v
 }
 
 omit [PartialOrder act] [PartialOrder test] in
 lemma branch_implies_node {α : Lpofin (Label act test)} {x : Node} :
-    ∀ φ : ↑α.branches, φ ≤ α.form x → x ∈ α.val.nodes := by
+    ∀ φ : ↑α.branches, φ.val.toForm ≤ α.form x → x ∈ α.val.nodes := by
   intro φ hle
-  have ⟨_, _, f, heq, _, hm_x⟩ := φ.property
-  have ⟨v, hsat⟩ := mk_form_sat f
+  have ⟨_, _, hm_x⟩ := φ.property
+  have ⟨v, hsat⟩ := φ.val.sat
   refine (α.val.property.form_dom x).mp ?_
-  use v; exact hle v (heq ▸ hsat)
+  use v; exact hle v hsat
 
 omit [PartialOrder act] [PartialOrder test] in
 lemma seq_nodes_finite {α β : Lpofin (Label act test)} {f : CopyFn α β} :
@@ -56,6 +57,7 @@ lemma seq_nodes_finite {α β : Lpofin (Label act test)} {f : CopyFn α β} :
   · exact α.branches_finite
   · intro φ; exact (f φ).property
 
+omit [PartialOrder act] [PartialOrder test] in
 lemma seq_rel_valid {α β : Lpofin (Label act test)} {f : CopyFn α β} :
     (seq_base α β f).rel.IsCausalityRel (seq_base α β f).nodes := by
   have h₁ := α.val.property
@@ -173,32 +175,28 @@ lemma seq_valid (α β : Lpofin (Label act test)) (f : CopyFn α β) :
         exact Exists.choose_spec (p := fun ψ ↦ x ∈ (f ψ).nodes) _
     · have hx' := branch_implies_node φ hx
       simp only [seq_base, nodes] at hlab
-      have ⟨t, _, g, heq, ⟨_, hstuck⟩, _⟩ := φ.property
-      have ⟨v, hsat⟩ := mk_form_sat g
-      rw [heq] at hx; have hform := hx v hsat
+      have ⟨_, hstuck, _⟩ := φ.property
+      have ⟨v, hsat⟩ := φ.val.sat
+      have hform := hx v hsat
       have : ¬ (∃ φ, x ∈ (f φ).nodes) := by
         intro ⟨ψ, hx⟩; exact Set.disjoint_left.mp (f.property ψ).2.1 hx' hx
       have := (dif_neg this).symm.trans hlab
-      exact hstuck v hsat ⟨⟨x, hx', this⟩, hform⟩
+      refine hstuck v hsat ⟨⟨x, hx', this, ?_⟩, hform⟩
+      exact ⟨φ, bot_le, hx⟩
   -- Formula Domain
   · intro x; constructor
-    · rintro ⟨v, hv⟩; by_cases hx : x ∈ α.nodes <;>
-      simp only [seq_base, Subtype.exists, hx, ↓reduceIte] at hv
-      · left; exact (α.val.property.form_dom x).mp ⟨v, hv⟩
-      · rcases hv with ⟨φ, hφ, _⟩; right
-        simp only [Set.mem_iUnion]
-        use φ; exact ((f φ).val.property.form_dom x).mp ⟨v, hφ⟩
+    · rintro ⟨_, hform | ⟨φ, hform, _⟩⟩
+      · left; exact (α.val.property.form_dom x).mp ⟨_, hform⟩
+      · right; refine Set.mem_iUnion.mpr ⟨φ, ?_⟩
+        exact((f φ).val.property.form_dom x).mp ⟨_, hform⟩
     · simp only [seq_base, nodes, Subtype.exists, Set.mem_union, Set.mem_iUnion]
       rintro (hx | ⟨φ, hφ, hx⟩)
-      · simp only [hx, ↓reduceIte]
-        exact (α.val.property.form_dom x).mpr hx
-      · have hx' : x ∉ α.val.nodes :=
-          Set.disjoint_right.mp (f.2 ⟨φ, hφ⟩).2.1 hx
-        simp only [hx', ↓reduceIte]
-        obtain ⟨v, hv⟩ := ((f ⟨φ, hφ⟩).val.property.form_dom x).mpr hx
-        have ⟨t, ht, g, heq, ⟨hconj, hstuck⟩, _⟩ := hφ
-        have ⟨v', hsat⟩ := mk_form_sat g
-        refine ⟨(v ∩ (f ⟨φ, hφ⟩).nodes) ∪ (v' ∩ α.nodes), ⟨φ, hφ⟩, ?_, ?_⟩
+      · have ⟨v, hform⟩ := (α.val.property.form_dom x).mpr hx
+        exact ⟨v, Or.inl hform⟩
+      · obtain ⟨v, hv⟩ := ((f ⟨φ, hφ⟩).val.property.form_dom x).mpr hx
+        have ⟨hconj, hstuck, _⟩ := hφ
+        have ⟨v', hsat⟩ := φ.sat
+        refine ⟨(v ∩ (f ⟨φ, hφ⟩).nodes) ∪ (v' ∩ α.nodes), Or.inr ⟨⟨φ, hφ⟩, ?_, ?_⟩⟩
         · refine (((f ⟨φ, hφ⟩).val.property.form _ hx).1 _ _ ?_).mp hv
           refine Set.disjoint_left.mpr ?_; intro y hy hrel
           rcases Set.mem_symmDiff.mp hy with ⟨hy, hy'⟩ | ⟨⟨hy, _⟩ | ⟨hy, ha⟩, hy'⟩
@@ -207,84 +205,94 @@ lemma seq_valid (α β : Lpofin (Label act test)) (f : CopyFn α β) :
             exact ((f _).val.property.rel_dom hrel).1
           · exact hy' hy
           · exact Set.disjoint_right.mp (f.property _).2.1 ((f _).val.property.rel_dom hrel).1 ha
-        · subst heq; simp only; intro y
-          have hy := tests_sub_nodes <| ht y.property
-          have hdep : (node_lit y (g y)).DependsOn {y.val} := node_lit_depends_on
-          refine (hdep _ _ ?_).mp <| hsat y
-          refine Set.disjoint_left.mpr ?_; rintro z hz rfl
-          rcases Set.mem_symmDiff.mp hz with ⟨hzv', hz⟩ | ⟨⟨hzv, hz⟩ | h, hzv'⟩
-          · simp only [Set.mem_union, Set.mem_inter_iff, not_or, not_and] at hz
-            apply hz.2 hzv' hy
-          · exact Set.disjoint_left.mp (f.property _).2.1 hy hz
+        · refine (φ.dependsOn _ _ ?_).mp hsat
+          refine Set.disjoint_left.mpr ?_; rintro z hsd hzt
+          rcases Set.mem_symmDiff.mp hsd with ⟨hzv', hz⟩ | ⟨⟨hzv, hz⟩ | h, hzv'⟩
+          · apply hz; right; exact ⟨hzv', tests_sub_nodes <| φ.tests_valid hzt⟩
+          · refine Set.disjoint_left.mp (f.property _).2.1 ?_ hz
+            exact tests_sub_nodes <| φ.tests_valid hzt
           · exact hzv' h.1
   -- Formula Properties
-  · rintro x (hx | hx) <;> refine ⟨?_, fun y hrel ↦ ?_⟩
-    · simp only [seq_base, if_pos hx]
-      refine Form.DependsOn.monotone _ ?_ (α.val.property.form _ hx).1
-      intro y hrel; left; exact hrel
-    · rcases hrel with hrel | ⟨φ, hrel | ⟨hform, hy⟩⟩
-      · have hy : y ∈ α.nodes := (α.val.property.rel_dom hrel).2
-        simp only [seq_base, if_pos hx, if_pos hy]
-        exact (α.val.property.form _ hx).2 _ hrel
-      · exfalso; refine Set.disjoint_left.mp (f.property φ).2.1 hx ?_
-        exact ((f φ).val.property.rel_dom hrel).1
-      · have hy' : y ∉ α.nodes :=
-          Set.disjoint_right.mp (f.property φ).2.1 hy
-        simp only [seq_base, if_pos hx, if_neg hy']
-        refine le_trans ?_ hform; intro v ⟨ψ, hsat, hψ⟩
-        have hy'' := ((f ψ).val.property.form_dom _).mp ⟨_, hsat⟩
-        have := not_not.mp (((f.property φ).2.2 ψ).mt (Set.not_disjoint_iff.mpr ⟨_, hy, hy''⟩))
-        subst this; exact hψ
-    · simp only [Set.mem_iUnion] at hx; have ⟨φ, hx⟩ := hx
-      have hx' : x ∉ α.nodes :=
-        Set.disjoint_right.mp (f.property φ).2.1 hx
-      simp only [seq_base, if_neg hx']
-      have :
-          (Form.sOr fun φ ↦ ((f φ).form x).and φ.val) =
-          ((f φ).form x).and φ.val := by
-        ext v; constructor
-        · intro ⟨ψ, hform⟩; by_cases heq : φ = ψ
-          · subst heq; exact hform
-          · exfalso; have := Set.disjoint_left.mp ((f.property φ).2.2 _ heq) hx
-            exact this (((f ψ).val.property.form_dom _).mp ⟨_, hform.1⟩)
-        · intro hform; exact ⟨φ, hform⟩
-      rw [this]
-      refine Form.DependsOn.monotone _
-        (?_ : ({ y | (f φ).rel y x } ∪ { y | φ.val ≤ α.form y }) ⊆ _)
-        ?_
-      · rintro y (hrel | hform)
-        · right; use φ; left; exact hrel
-        · right; use φ; right; exact ⟨hform, hx⟩
-      · refine Form.DependsOn.and ?_ ?_
-        · exact ((f φ).val.property.form  _ hx).1
-        · have ⟨s, ht, g, heq, ⟨hconj, _⟩, _⟩ := φ.property
-          rw [heq]
-          refine Form.DependsOn.monotone _
-            (?_ : (⋃ z : ↑s, { z.val }) ⊆ _)
-            ?_
-          · rintro z ⟨_, ⟨y, rfl⟩, rfl⟩ v hform
-            exact hconj _ hform y
-          · exact Form.DependsOn.sAnd fun _ ↦ node_lit_depends_on
-    · rcases hrel with (hrel | ⟨φ, hrel | ⟨hform, hy⟩⟩)
-      · have ⟨hx, hy⟩ := α.val.property.rel_dom hrel
-        refine le_of_eq_of_le (if_pos hy) ?_
-        refine le_of_le_of_eq ?_ (if_pos hx).symm
-        exact (α.val.property.form _ hx).2 _ hrel
-      · have ⟨hx, hy⟩ := (f φ).val.property.rel_dom hrel
-        have hx' := Set.disjoint_right.mp (f.property φ).2.1 hx
-        have hy' := Set.disjoint_right.mp (f.property φ).2.1 hy
-        refine le_of_eq_of_le (if_neg hy') ?_
-        refine le_of_le_of_eq ?_ (if_neg hx').symm
-        intro v ⟨ψ, hform, hφ⟩
-        have hy'' := ((f ψ).val.property.form_dom _).mp ⟨_, hform⟩
-        have := not_not.mp (((f.property φ).2.2 ψ).mt (Set.not_disjoint_iff.mpr ⟨_, hy, hy''⟩))
-        subst this; refine ⟨φ, ?_, hφ⟩
-        exact ((f φ).val.property.form _ hx).2 _ hrel _ hform
-      · exfalso; simp only [Set.mem_iUnion] at hx
-        have ⟨ψ, hx⟩ := hx; refine Set.disjoint_right.mp (f.property ψ).2.1 hx ?_
-        have ⟨t, _, g, heq, _⟩ := φ.property; have ⟨v, hsat⟩ := mk_form_sat g
-        rw [heq] at hform; refine (α.val.property.form_dom _).mp ⟨v, ?_⟩
-        exact hform _ hsat
+  · rintro x (hx | ⟨_, ⟨φ, rfl⟩, hx⟩) <;> refine ⟨?_, fun y hrel ↦ ?_⟩
+    · refine Form.DependsOn.or ?_ ?_
+      · exact (α.val.property.form _ hx).1
+      · intro v v' _; ext; constructor; all_goals
+          intro ⟨φ, hc, _⟩; exfalso
+          refine ((f φ).val.property.form_dom x).mp.mt ?_ ⟨_, hc⟩
+          exact Set.disjoint_left.mp (f.property φ).2.1 hx
+    · rintro v (hform | ⟨φ, hform, hφ⟩)
+      · left; rcases hrel with hrel | ⟨φ, hrel | ⟨_, hy'⟩⟩
+        · have hx := α.val.property.rel_dom hrel |>.1
+          exact (α.val.property.form _ hx).2 _ hrel _ hform
+        · exfalso; refine Set.disjoint_left.mp (f.property φ).2.1 hx ?_
+          exact (f φ).val.property.rel_dom hrel |>.1
+        · exfalso; refine Set.disjoint_left.mp (f.property φ).2.1 ?_ hy'
+          exact (α.val.property.form_dom y).mp ⟨_, hform⟩
+      · have hy := ((f φ).val.property.form_dom y).mp ⟨_, hform⟩
+        rcases hrel with hrel | ⟨ψ, h⟩
+        · exfalso; refine Set.disjoint_right.mp (f.property φ).2.1 hy ?_
+          exact α.val.property.rel_dom hrel |>.2
+        · have : ψ = φ := by
+            by_contra hne
+            refine Set.disjoint_right.mp ((f.property ψ).2.2 _ hne) hy ?_
+            rcases h with hrel | ⟨_, hy⟩
+            · exact (f ψ).val.property.rel_dom hrel |>.2
+            · exact hy
+          subst this; rcases h with hrel | ⟨himp, hy⟩
+          · right
+            have ⟨hx, hy'⟩ := (f ψ).val.property.rel_dom hrel
+            refine ⟨ψ, ?_, hφ⟩
+            exact ((f ψ).val.property.form _ hx).2 _ hrel _ hform
+          · left; exact himp _ hφ
+    · refine Form.DependsOn.or ?_ ?_
+      · intro v v' _; ext; constructor; all_goals
+          intro hform; exfalso
+          refine (α.val.property.form_dom x).mp.mt ?_ ⟨_, hform⟩
+          exact Set.disjoint_right.mp (f.property φ).2.1 hx
+      · have heq :
+            (fun y ↦ ∃ φ, (f φ).rel y x ∨ φ.val.toForm ≤ α.form y ∧ x ∈ (f φ).nodes) =
+            ⋃ φ : ↑α.branches,
+              { y | (f φ).rel y x } ∪ { y | φ.val.toForm ≤ α.form y ∧ x ∈ (f φ).nodes } := by
+          ext z; refine Iff.trans ?_ Set.mem_iUnion.symm
+          refine exists_congr fun φ ↦ Iff.refl _
+        rw [heq]; refine Form.DependsOn.sOr fun ψ ↦ ?_
+        by_cases heq : ψ = φ
+        · subst heq; refine (Form.DependsOn.and ?_ ?_)
+          · exact ((f ψ).val.property.form _ hx).1
+          · refine ψ.val.dependsOn.monotone _ ?_
+            intro y hy; have ⟨h, _⟩ := ψ.property; exact ⟨h _ hy, hx⟩
+        · intro v v' _; ext; constructor; all_goals
+            intro ⟨hform, _⟩; exfalso
+            refine Set.disjoint_right.mp ((f.property ψ).2.2 _ heq) hx ?_
+            exact ((f ψ).val.property.form_dom _).mp ⟨_, hform⟩
+    · rcases hrel with hrel | ⟨ψ, h⟩
+      · exfalso; refine Set.disjoint_right.mp (f.property φ).2.1 hx ?_
+        exact α.val.property.rel_dom hrel |>.1
+      · have : ψ = φ := by
+          by_contra hne
+          rcases h with hrel | ⟨himp, _⟩
+          · refine Set.disjoint_right.mp ((f.property ψ).2.2 _ hne) hx ?_
+            exact (f ψ).val.property.rel_dom hrel |>.1
+          · refine Set.disjoint_right.mp (f.property φ).2.1 hx ?_
+            have ⟨v, hsat⟩ := ψ.val.sat
+            exact (α.val.property.form_dom x).mp ⟨v, himp _ hsat⟩
+        subst this; rcases h with hrel | ⟨himp, hform⟩
+        · rintro v (hform | ⟨φ, hform, hψ⟩)
+          · exfalso; have hy := ((f ψ).val.property.rel_dom hrel).2
+            refine Set.disjoint_right.mp (f.property ψ).2.1 hy ?_
+            exact (α.val.property.form_dom _).mp ⟨_, hform⟩
+          · have : ψ = φ := by
+              by_contra hne; have hy := (f ψ).val.property.rel_dom hrel |>.2
+              refine Set.disjoint_left.mp ((f.property ψ).2.2 _ hne) hy ?_
+              exact ((f φ).val.property.form_dom _).mp ⟨_, hform⟩
+            subst this
+            right; refine ⟨ψ, ?_, hψ⟩
+            exact ((f ψ).val.property.form _ hx).2 _ hrel _ hform
+        · exfalso; refine Set.disjoint_right.mp (f.property ψ).2.1 hx ?_
+          refine (α.val.property.form_dom x).mp ?_
+          have ⟨v, hsat⟩ := ψ.val.sat
+          exact ⟨v, himp _ hsat⟩
+
 
 noncomputable def seq (α β : Lpofin (Label act test)) (f : CopyFn α β) :
     Lpofin (Label act test) := {
@@ -307,7 +315,7 @@ lemma seq_monotone {α α' β β' : Lpofin (Label act test)} {f : CopyFn α β} 
     · intro φ hφ x hx; right
       have hφ' := branches_monotone hle₁ hφ
       simp only [Set.mem_iUnion, Subtype.exists]
-      exact ⟨φ, hφ', (hext ⟨φ, hφ⟩).nodes hx⟩
+      exact ⟨φ.up_cast hle₁, hφ', (hext ⟨φ, hφ⟩).nodes hx⟩
   · rintro x (hx | hx) y hyx
     · rcases hyx with (hyx | ⟨ψ, hyx | ⟨hx', hy⟩⟩)
       · left; exact hle₁.downcl x hx y hyx
@@ -320,22 +328,23 @@ lemma seq_monotone {α α' β β' : Lpofin (Label act test)} {f : CopyFn α β} 
         exact Set.disjoint_left.mp (g.property _).2.1
           (α'.val.property.rel_dom hyx).2
           hx'
-      · by_cases heq : ψ = ⟨φ.val, branches_monotone hle₁ φ.property⟩
+      · by_cases heq : ψ = ⟨φ.val.up_cast hle₁, branches_monotone hle₁ φ.property⟩
         · subst heq; rcases hyx with hyx | ⟨hy, hx'⟩
           · right; refine Set.mem_iUnion.mpr ⟨φ, ?_⟩;
             exact (hext φ).downcl x hx y hyx
           · left
-            have ⟨t, _, g, heq, ⟨_, hstk⟩, _⟩ := φ.property
-            have ⟨v, hsat⟩ := mk_form_sat g
+            have ⟨_, hstk, _⟩ := φ.property
+            have ⟨v, hsat⟩ := φ.val.sat
             have hy' : y ∈ α'.nodes := by
               refine (α'.val.property.form_dom _).mp ?_
-              rw [heq] at hy; exact ⟨v, hy _ hsat⟩
+              exact ⟨v, hy _ hsat⟩
             refine or_iff_not_imp_right.mp (hle₁.succ _ hy') ?_
             intro ⟨z, hz, hrel⟩
-            refine not_exists.mp (hstk _ hsat) ⟨_, hz⟩ ?_
-            refine (congrFun (hle₁.form _ hz.1) _).mpr ?_
-            refine (α'.val.property.form _ (hle₁.nodes hz.1)).2 _ hrel _ ?_
-            rw [heq] at hy; exact hy _ hsat
+            refine not_exists.mp (hstk _ hsat) ⟨z, hz.1, hz.2, ?_⟩ ?_
+            · sorry
+            · refine (congrFun (hle₁.form _ hz.1) _).mpr ?_
+              refine (α'.val.property.form _ (hle₁.nodes hz.1)).2 _ hrel _ ?_
+              exact hy _ hsat
         · exfalso
           refine Set.disjoint_left.mp ((g.property ψ).2.2 _ heq)
               ?_
@@ -346,15 +355,14 @@ lemma seq_monotone {α α' β β' : Lpofin (Label act test)} {f : CopyFn α β} 
   · intro x hx y hy; ext; constructor
     · rintro (hrel | ⟨φ, h⟩)
       · left; exact le_rel hle₁ hrel
-      · right; refine ⟨⟨φ.val, branches_monotone hle₁ φ.property⟩, ?_⟩
+      · right; refine ⟨⟨φ.val.up_cast hle₁, branches_monotone hle₁ φ.property⟩, ?_⟩
         rcases h with (hrel | ⟨hform, hy'⟩)
         · left; exact le_rel (hext _) hrel
         · right; refine ⟨?_, (hext _).nodes hy'⟩
           refine le_of_le_of_eq hform (hle₁.form _ ?_)
           refine (α.val.property.form_dom _).mp ?_
-          have ⟨t, _, g, heq, _⟩ := φ.property
-          have ⟨v, hsat⟩ := mk_form_sat g
-          rw [heq] at hform; exact ⟨v, hform _ hsat⟩
+          have ⟨v, hsat⟩ := φ.val.sat
+          exact ⟨v, hform _ hsat⟩
     · simp only [Lpo.nodes, seq, seq_base, nodes, Set.mem_union, Set.mem_iUnion, Lpo.rel] at *
       obtain (hx | ⟨φ, hx⟩) := hx <;>
       obtain (hy | ⟨ψ, hy⟩) := hy <;>
@@ -369,7 +377,9 @@ lemma seq_monotone {α α' β β' : Lpofin (Label act test)} {f : CopyFn α β} 
         exact Set.disjoint_left.mp (g.property _).2.1 (hle₁.nodes hx) hx'
       · refine Or.inr ⟨ψ, Or.inr ⟨?_, hy⟩⟩
         refine le_of_eq_of_le ?_ (le_of_le_of_eq hform ?_)
-        · refine congrArg Subtype.val (not_not.mp (((g.property φ').2.2 ⟨ψ.val, ?_⟩).mt ?_)).symm
+        · conv => lhs; exact (PathCond.cast_toForm (hle := hle₁)).symm
+          refine congrArg _ ?_
+          refine congrArg Subtype.val (not_not.mp (((g.property φ').2.2 ⟨ψ.val.up_cast hle₁, ?_⟩).mt ?_)).symm
           · exact branches_monotone hle₁ ψ.property
           · exact Set.not_disjoint_iff.mpr ⟨y, hy', (hext _).nodes hy⟩
         · symm; exact hle₁.form _ hx
@@ -382,23 +392,22 @@ lemma seq_monotone {α α' β β' : Lpofin (Label act test)} {f : CopyFn α β} 
         exact Set.disjoint_left.mp (g.property _).2.1 hx' ((hext _).nodes hx)
       · refine Or.inr ⟨φ, Or.inl ?_⟩
         have ⟨hx', hy'⟩ := (g _).val.property.rel_dom hrel
-        have heq : φ.val = φ'.val := by
-          refine congrArg Subtype.val (not_not.mp (((g.property φ').2.2 ⟨φ.val, ?_⟩).mt ?_)).symm
+        have heq : φ.val.up_cast hle₁ = φ'.val := by
+          refine congrArg Subtype.val (not_not.mp (((g.property φ').2.2 ⟨φ.val.up_cast hle₁, ?_⟩).mt ?_)).symm
           · exact branches_monotone hle₁ φ.property
           · exact Set.not_disjoint_iff.mpr ⟨x, hx', (hext _).nodes hx⟩
         have : φ = ψ := by
-          ext1; rw [heq]
-          refine congrArg Subtype.val (not_not.mp (((g.property φ').2.2 ⟨ψ.val, ?_⟩).mt ?_))
-          · exact branches_monotone hle₁ ψ.property
-          · exact Set.not_disjoint_iff.mpr ⟨y, hy', (hext _).nodes hy⟩
+          rcases φ' with ⟨φ', _⟩; subst heq; sorry
+          -- refine not_not.mp (((g.property _).2.2 ⟨ψ.val.up_cast hle₁, ?_⟩).mt ?_)
+          -- · exact branches_monotone hle₁ ψ.property
+          -- · exact Set.not_disjoint_iff.mpr ⟨y, hy', (hext _).nodes hy⟩
         subst this; refine ((hext φ).rel _ hx _ hy).mpr ?_
-        · have {h} : ⟨φ.val, h⟩ = φ' := by ext1; exact heq
+        · have {h} : ⟨φ.val.up_cast hle₁, h⟩ = φ' := by ext1; exact heq
           rw [this]; exact hrel
       · exfalso; refine Set.disjoint_left.mp (g.property _).2.1 ?_ ((hext _).nodes hx)
         refine (α'.val.property.form_dom _).mp ?_
-        have ⟨t, _, g, heq, _⟩ := φ'.property
-        have ⟨v, hsat⟩ := mk_form_sat g
-        rw [heq] at hform; exact ⟨v, hform _ hsat⟩
+        have ⟨v, hsat⟩ := φ'.val.sat
+        exact ⟨v, hform _ hsat⟩
   · intro x; by_cases hx : x ∈ (α.seq β f).nodes
     · rcases hx with hx | hx
       · have hx' : x ∈ α'.nodes := hle₁.nodes hx
@@ -410,7 +419,7 @@ lemma seq_monotone {α α' β β' : Lpofin (Label act test)} {f : CopyFn α β} 
         exact hle₁.lab x
       · simp only [Set.mem_iUnion] at hx
         have ⟨φ, hf⟩ := hx; have hg := (hext φ).nodes hf
-        have hx' : ∃ φ, x ∈ (g φ).nodes := ⟨⟨φ.val, _⟩, hg⟩
+        have hx' : ∃ φ, x ∈ (g φ).nodes := ⟨⟨φ.val.up_cast hle₁, _⟩, hg⟩
         simp only [Lpo.lab, seq, seq_base, dif_pos hx, dif_pos hx']
         refine le_of_le_of_eq ((hext _).lab x) ?_
         refine congrArg₂ Lpofin.lab (congrArg _ ?_) rfl
@@ -420,35 +429,37 @@ lemma seq_monotone {α α' β β' : Lpofin (Label act test)} {f : CopyFn α β} 
     · exact le_of_eq_of_le ((α.seq β f).val.property.lab_dom _ hx) bot_le
   · rintro x (hx | hx)
     · have hx' := hle₁.nodes hx
-      simp only [Lpo.form, Lpofin.nodes, Lpo.nodes, seq, seq_base] at *
-      simp only [hx, hx', ↓reduceIte]; exact hle₁.form x hx
+      ext v; refine or_congr ?_ ?_
+      · apply iff_iff_eq.mpr; exact congrFun (hle₁.form _ hx) _
+      · sorry
     · rcases Set.mem_iUnion.mp hx with ⟨φ, h⟩
-      simp only [Lpo.form, Lpofin.nodes, Lpo.nodes, seq, seq_base] at *
-      have hx₁ := Set.disjoint_right.mp (f.property φ).2.1 h
-      have hx₂ := Set.disjoint_right.mp (g.property _).2.1 ((hext φ).nodes h)
-      simp only [Lpofin.nodes, Lpo.nodes] at hx₁
-      simp only [Lpofin.nodes, Lpo.nodes] at hx₂
-      simp only [hx₁, ↓reduceIte, hx₂]
-      ext v; constructor
-      · intro ⟨ψ, hψ, hφ⟩
-        have heq : φ = ψ := by
-          by_contra hc
-          have hd := (f.property φ).2.2 ψ hc
-          have hx := Set.disjoint_left.mp hd h
-          exact ((f ψ).val.property.form_dom x).mp.mt hx ⟨v, hψ⟩
-        subst heq; exact ⟨_, (congrFun ((hext _).form _ h) _).mp hψ, hφ⟩
-      · intro ⟨ψ, hform, hψ⟩
-        have heq : ψ.val = φ.val := by
-          have hx' := ((g ψ).val.property.form_dom _).mp ⟨_, hform⟩
-          refine congrArg Subtype.val (not_not.mp (((g.property ψ).2.2 ⟨φ, ?_⟩).mt ?_))
-          · exact branches_monotone hle₁ φ.property
-          · exact Set.not_disjoint_iff.mpr ⟨x, hx', (hext _).nodes h⟩
-        refine ⟨φ, ?_, ?_⟩
-        · refine (congrFun ?_ _).mpr hform
-          refine ((hext φ).form _ h).trans ?_
-          have {h} : ⟨φ.val, h⟩ = ψ := by ext1; exact heq.symm
-          rw [this]; rfl
-        · rw [← heq]; exact hψ
+      sorry
+      -- simp only [Lpo.form, Lpofin.nodes, Lpo.nodes, seq, seq_base] at *
+      -- have hx₁ := Set.disjoint_right.mp (f.property φ).2.1 h
+      -- have hx₂ := Set.disjoint_right.mp (g.property _).2.1 ((hext φ).nodes h)
+      -- simp only [Lpofin.nodes, Lpo.nodes] at hx₁
+      -- simp only [Lpofin.nodes, Lpo.nodes] at hx₂
+      -- simp only [hx₁, ↓reduceIte, hx₂]
+      -- ext v; constructor
+      -- · intro ⟨ψ, hψ, hφ⟩
+      --   have heq : φ = ψ := by
+      --     by_contra hc
+      --     have hd := (f.property φ).2.2 ψ hc
+      --     have hx := Set.disjoint_left.mp hd h
+      --     exact ((f ψ).val.property.form_dom x).mp.mt hx ⟨v, hψ⟩
+      --   subst heq; exact ⟨_, (congrFun ((hext _).form _ h) _).mp hψ, hφ⟩
+      -- · intro ⟨ψ, hform, hψ⟩
+      --   have heq : ψ.val = φ.val := by
+      --     have hx' := ((g ψ).val.property.form_dom _).mp ⟨_, hform⟩
+      --     refine congrArg Subtype.val (not_not.mp (((g.property ψ).2.2 ⟨φ, ?_⟩).mt ?_))
+      --     · exact branches_monotone hle₁ φ.property
+      --     · exact Set.not_disjoint_iff.mpr ⟨x, hx', (hext _).nodes h⟩
+      --   refine ⟨φ, ?_, ?_⟩
+      --   · refine (congrFun ?_ _).mpr hform
+      --     refine ((hext φ).form _ h).trans ?_
+      --     have {h} : ⟨φ.val, h⟩ = ψ := by ext1; exact heq.symm
+      --     rw [this]; rfl
+      --   · rw [← heq]; exact hψ
   · simp only [Lpo.nodes, seq, seq_base, Set.mem_union, Set.mem_iUnion, Lpo.bots, Lpo.rel, Lpo.lab]
     rintro x (hx | ⟨φ, hx⟩)
     · rcases hle₁.succ _ hx with (hx' | ⟨z, hz, hrel⟩)
@@ -457,30 +468,31 @@ lemma seq_monotone {α α' β β' : Lpofin (Label act test)} {f : CopyFn α β} 
         refine (dif_neg ?_).trans hz.2
         intro ⟨φ, hz'⟩
         exact Set.disjoint_left.mp (f.property φ).2.1 hz.1 hz'
-    · by_cases hφ : φ.val ∈ α.branches
-      · rcases (hext ⟨_, hφ⟩).succ _ hx with (hx' | ⟨z, hz, hrel⟩)
-        · left; right; exact ⟨_, hx'⟩
-        · right; refine ⟨z, ⟨Or.inr ⟨_, hz.1⟩, ?_⟩, Or.inr ⟨φ, Or.inl hrel⟩⟩
-          refine (dif_pos ⟨_, hz.1⟩).trans ?_
-          have {ψ} : (f ψ).lab z = ⊥ := by
-            by_cases heq : ψ = ⟨φ.val, hφ⟩
-            · subst heq; exact hz.2
-            · refine (f ψ).val.property.lab_dom _ ?_
-              exact Set.disjoint_right.mp ((f.property _).2.2 _ heq) hz.1
-          exact this
-      · right
-        have ⟨t, _, g, heq, ⟨himp, hstk⟩, hmax⟩ := φ.property
-        rw [le_branches hle₁] at hφ
-        have h := φ.property
-        have ⟨v', hform⟩ := not_forall.mp ((Set.mem_inter h).mt hφ)
-        have ⟨hv, hform⟩ := Classical.not_imp.mp hform
-        have ⟨⟨z, hz⟩, hform⟩ := not_not.mp hform
-        by_cases hz' : z ∈ t
-        · refine ⟨z, ⟨Or.inl hz.1, ?_⟩, Or.inr ⟨φ, Or.inr ⟨?_, hx⟩⟩⟩
-          · refine (dif_neg ?_).trans hz.2
-            intro ⟨φ, hz'⟩; exact Set.disjoint_left.mp (f.property φ).2.1 hz.1 hz'
-          · rw [heq]; intro v hv; exact himp _ hv ⟨_, hz'⟩
-        · exfalso; sorry
+    · sorry
+      -- by_cases hφ : φ.val ∈ α.branches
+      -- · rcases (hext ⟨_, hφ⟩).succ _ hx with (hx' | ⟨z, hz, hrel⟩)
+      --   · left; right; exact ⟨_, hx'⟩
+      --   · right; refine ⟨z, ⟨Or.inr ⟨_, hz.1⟩, ?_⟩, Or.inr ⟨φ, Or.inl hrel⟩⟩
+      --     refine (dif_pos ⟨_, hz.1⟩).trans ?_
+      --     have {ψ} : (f ψ).lab z = ⊥ := by
+      --       by_cases heq : ψ = ⟨φ.val, hφ⟩
+      --       · subst heq; exact hz.2
+      --       · refine (f ψ).val.property.lab_dom _ ?_
+      --         exact Set.disjoint_right.mp ((f.property _).2.2 _ heq) hz.1
+      --     exact this
+      -- · right
+      --   have ⟨t, _, g, heq, ⟨himp, hstk⟩, hmax⟩ := φ.property
+      --   rw [le_branches hle₁] at hφ
+      --   have h := φ.property
+      --   have ⟨v', hform⟩ := not_forall.mp ((Set.mem_inter h).mt hφ)
+      --   have ⟨hv, hform⟩ := Classical.not_imp.mp hform
+      --   have ⟨⟨z, hz⟩, hform⟩ := not_not.mp hform
+      --   by_cases hz' : z ∈ t
+      --   · refine ⟨z, ⟨Or.inl hz.1, ?_⟩, Or.inr ⟨φ, Or.inr ⟨?_, hx⟩⟩⟩
+      --     · refine (dif_neg ?_).trans hz.2
+      --       intro ⟨φ, hz'⟩; exact Set.disjoint_left.mp (f.property φ).2.1 hz.1 hz'
+      --     · rw [heq]; intro v hv; exact himp _ hv ⟨_, hz'⟩
+      --   · exfalso; sorry
           --  rw [heq] at hv; refine hstk _ hv ?_
           -- have : z ∉ α'.tests := by
           --   intro hc; refine hmax hz' hc ⟨?_, ?_, ?_⟩ (b := true)
