Pom/Lpo/Operations/Seq/PathCond.lean
@@ -1,0 +1,202 @@
+import Mathlib.Data.Finite.Sigma
+
+import Pom.Lpo.Linearization.Label
+import Pom.Lpo.Operations.Seq.Equiv
+import Pom.Lpo.Order.FinApprox
+
+namespace Lpofin
+
+variable {act test : Type}
+
+def isTest (α : Lpofin (Label act test)) (x : Node) : Prop := Label.isTest (α.lab x)
+
+def tests (α : Lpofin (Label act test)) : Set Node := { x | α.isTest x }
+
+lemma tests_sub_nodes {α : Lpofin (Label act test)} : α.tests ⊆ α.nodes := by
+  intro x hx
+  refine (α.val.property.lab_dom x).mt ?_ |> not_not.mp
+  have ⟨b, hlab⟩ := (Label.isTest_iff _).mp hx
+  conv => arg 1; lhs; exact hlab
+  exact Label.test_ne_bot _
+
+structure PathCond (α : Lpofin (Label act test)) where
+  tests : Set Node
+  truth : ↑tests → Bool
+  tests_valid : tests ⊆ α.tests
+attribute [ext] PathCond
+
+namespace PathCond
+
+instance finite (α : Lpofin (Label act test)) : Finite (PathCond α) := by
+  have hfin : Finite ↑α.tests.powerset := by
+    refine (α.property.subset ?_).powerset.to_subtype
+    intro x hx; exact tests_sub_nodes hx
+  refine @Finite.of_injective _ (Σ (s : ↑α.tests.powerset), ↑s.val → Bool) ?_
+    (fun φ ↦ ⟨⟨φ.tests, φ.tests_valid⟩, φ.truth⟩) ?_
+  · refine @Finite.instSigma _ _ hfin ?_
+    intro s; refine @Pi.finite _ _ ?_ _
+    refine Set.Finite.to_subtype (α.property.subset ?_)
+    exact s.property.trans tests_sub_nodes
+  · intro φ ψ heq; simp only [Sigma.mk.injEq, Subtype.mk.injEq] at heq
+    ext1
+    · exact heq.1
+    · exact heq.2
+
+def empty {α : Lpofin (Label act test)} : PathCond α := {
+  tests := ∅
+  truth := fun ⟨_, h⟩ ↦ False.elim <| Set.notMem_empty _ h
+  tests_valid := Set.empty_subset _
+}
+
+instance {α : Lpofin (Label act test)} : Bot (PathCond α) where
+  bot := empty
+
+def toForm {α : Lpofin (Label act test)} (φ : PathCond α) : Form Node :=
+  Form.sAnd fun x ↦ if φ.truth x then Form.literal x.val else (Form.literal x.val).not
+
+def extend {α : Lpofin (Label act test)} (φ : PathCond α) {x : Node} (hx : α.isTest x) (b : Bool) :
+    PathCond α := {
+  tests := φ.tests.insert x
+  truth := fun ⟨z, hz⟩ ↦ if h : z = x then b else φ.truth ⟨z, Set.mem_of_mem_insert_of_ne hz h⟩
+  tests_valid := by
+    intro z hz; rcases Set.mem_insert_iff.mp hz with rfl | hz
+    · exact hx
+    · exact φ.tests_valid hz
+}
+
+open Classical in
+noncomputable def union {α : Lpofin (Label act test)} (φ ψ : PathCond α) : PathCond α := {
+  tests := φ.tests ∪ ψ.tests
+  truth := fun ⟨z, hz⟩ ↦
+    if h : z ∈ φ.tests then φ.truth ⟨z, h⟩ else ψ.truth ⟨z, Or.resolve_left hz h⟩
+  tests_valid := Set.union_subset φ.tests_valid ψ.tests_valid
+}
+
+instance {α : Lpofin (Label act test)} : LE (PathCond α) where
+  le φ ψ :=
+    ∃ (h : φ.tests ⊆ ψ.tests),
+      ∀ x : ↑φ.tests, φ.truth x = ψ.truth ⟨x.val, h x.property⟩
+
+instance {α : Lpofin (Label act test)} : Preorder (PathCond α) where
+  le_refl φ := ⟨subset_refl _, fun _ ↦ rfl⟩
+  le_trans _ _ _ := by
+    intro ⟨hsub₁, heq₁⟩ ⟨hsub₂, heq₂⟩
+    refine ⟨hsub₁.trans hsub₂, ?_⟩; intro x
+    exact (heq₁ x).trans <| heq₂ ⟨x.val, hsub₁ x.property⟩
+
+instance {α : Lpofin (Label act test)} : OrderBot (PathCond α) where
+  bot_le _ := ⟨Set.empty_subset _, fun x ↦ False.elim x.property⟩
+
+lemma extend_le {α : Lpofin (Label act test)} (φ : PathCond α) {x : Node}
+    (hx : x ∉ φ.tests) (ht : α.isTest x) (b : Bool) : φ ≤ φ.extend ht b := by
+  refine ⟨Set.subset_insert _ _, ?_⟩
+  intro z; have hz : z ≠ x := by rintro rfl; exact hx z.property
+  symm; exact dif_neg hz
+
+lemma le_union_left {α : Lpofin (Label act test)} {φ ψ : PathCond α} :
+    φ ≤ φ.union ψ := by
+  refine ⟨Set.subset_union_left, ?_⟩; intro x; symm; exact dif_pos x.property
+
+lemma le_union_right {α : Lpofin (Label act test)} {φ ψ : PathCond α}
+    (h : ∀ {x}, ∀ hx : x ∈ φ.tests ∩ ψ.tests,
+      φ.truth ⟨x, Set.inter_subset_left hx⟩ = ψ.truth ⟨x, Set.inter_subset_right hx⟩) :
+    ψ ≤ φ.union ψ := by
+  refine ⟨Set.subset_union_right, ?_⟩; intro x; by_cases hx : x.val ∈ φ.tests
+  · conv => rhs; exact dif_pos hx
+    symm; exact h ⟨hx, x.property⟩
+  · symm; exact dif_neg hx
+
+lemma toForm_antitone {α : Lpofin (Label act test)} : Antitone (toForm (α := α)) := by
+  intro φ ψ ⟨hsub, heq⟩ v hψ x
+  rw [heq x]; exact hψ ⟨x.val, hsub x.property⟩
+
+lemma truth_iff_mem {α : Lpofin (Label act test)} (φ : PathCond α) {v : Set Node}
+    (hsat : φ.toForm v) {x : φ.tests} : φ.truth x = true ↔ x.val ∈ v := by
+  constructor
+  · intro h; exact hsat x |> (congrFun (if_pos h) _).mp
+  · intro h; by_contra ht
+    apply hsat x |> (congrFun (if_neg ht) _).mp; exact h
+
+lemma dependsOn {α : Lpofin (Label act test)} (φ : PathCond α) : φ.toForm.DependsOn φ.tests := by
+  rw [← Set.iUnion_of_singleton_coe φ.tests]
+  refine Form.DependsOn.sAnd fun x ↦ ?_; cases φ.truth x
+  · exact Form.DependsOn.literal.not
+  · exact Form.DependsOn.literal
+
+lemma sat {α : Lpofin (Label act test)} (φ : PathCond α) : φ.toForm.sat := by
+  use { x | ∃ (hx : x ∈ φ.tests), φ.truth ⟨x, hx⟩ = true }
+  intro x; cases heq : φ.truth x
+  · apply not_exists.mpr; intro hx
+    simp only [Subtype.coe_eta, heq, Bool.false_eq_true, not_false_eq_true]
+  · exact ⟨x.property, heq⟩
+
+def up_cast [Preorder act] [Preorder test] {α β : Lpofin (Label act test)} (φ : PathCond α)
+    (hle : α ≤ β) : PathCond β := {
+  tests := φ.tests
+  truth := φ.truth
+  tests_valid := by
+    apply φ.tests_valid.trans
+    intro x hx; have ⟨_, hlab⟩ := (Label.isTest_iff _).mp hx
+    have ⟨_, h, _⟩ := lab_is_test_le (le_of_eq_of_le hlab.symm <| hle.lab x)
+    exact (Label.isTest_iff _).mpr ⟨_, h⟩
+}
+
+lemma cast_toForm [Preorder act] [Preorder test] {α β : Lpofin (Label act test)} {φ : PathCond α}
+    {hle : α ≤ β} : (φ.up_cast hle).toForm = φ.toForm := by
+  ext v; refine forall_congr' ?_; intro x; rfl
+
+def permute {α : Lpofin (Label act test)} {Y : Set Node} (φ : PathCond α) (e : α.nodes ≃ Y) :
+    PathCond (α.permute e) :=
+  let e' := e.restrict (φ.tests_valid.trans tests_sub_nodes)
+  {
+    tests := Set.range fun x ↦ (e' x).val
+    truth := fun x ↦ φ.truth (e'.symm x)
+    tests_valid := by
+      rintro _ ⟨x, rfl⟩
+      have ⟨b, hlab⟩ := (Label.isTest_iff _).mp (φ.tests_valid x.property)
+      refine (Label.isTest_iff _).mpr ⟨b, ?_⟩
+      have ⟨x', heq⟩ := Set.mem_range.mp (e' x).property
+      simp only; rw [← heq]
+      refine (dif_pos ?_).trans ?_
+      · exact Subtype.coe_prop _
+      · conv => lhs; arg 2; arg 1; exact e.symm_apply_apply _
+        simp only [Equiv.restrict, Equiv.coe_fn_mk, e'] at heq
+        apply Subtype.val_injective at heq
+        apply e.injective at heq; simp only [Subtype.mk.injEq] at heq
+        rw [heq]; exact hlab
+  }
+
+lemma implies_weaken {α : Lpofin (Label act test)} {φ ψ : PathCond α} {P : Form Node}
+    (hext : φ ≤ ψ) (himp : ψ.toForm ≤ P)
+    (hdep : P.DependsOn (ψ.tests \ φ.tests).compl) :
+    φ.toForm ≤ P := by
+  intro v hφ; have ⟨v', hψ'⟩ := ψ.sat; have ⟨hsub, htr⟩ := hext
+  let u := (v ∩ (ψ.tests \ φ.tests).compl) ∪ (v' ∩ (ψ.tests \ φ.tests))
+  have hψ : ψ.toForm u := by
+    subst u; refine (ψ.dependsOn _ _ ?_).mp hψ'
+    refine Set.disjoint_left.mpr ?_; intro x hsd ht
+    rcases Set.mem_symmDiff.mp hsd with ⟨hv', h'⟩ | ⟨h | h, hv'⟩
+    · apply h'; clear h'; by_cases ht' : x ∈ ψ.tests \ φ.tests
+      · right; exact ⟨hv', ht'⟩
+      · left; refine ⟨?_, ht'⟩
+        have hxt := (Set.mem_sdiff_of_mem ht).mt ht' |> not_not.mp
+        apply (φ.truth_iff_mem hφ (x := ⟨_, hxt⟩)).mp
+        rw [htr ⟨_, hxt⟩]
+        exact (ψ.truth_iff_mem hψ' (x := ⟨_, ht⟩)).mpr hv'
+    · apply Set.mem_compl h.2; refine ⟨ht, ?_⟩
+      intro hxt;
+      apply (ψ.truth_iff_mem hψ' (x := ⟨_, ht⟩)).mp.mt hv'
+      rw [← htr ⟨_, hxt⟩]
+      exact (φ.truth_iff_mem hφ (x := ⟨_, hxt⟩)).mpr h.1
+    · exact hv' h.1
+  apply hdep.restrict.mpr
+  refine (congrArg P ?_).mp <| hdep.restrict.mp <| himp _ hψ; subst u
+  ext x; constructor
+  · rintro ⟨h | h, h'⟩
+    · exact h
+    · exfalso; exact h' h.2
+  · intro h; exact ⟨Or.inl h, h.2⟩
+
+end PathCond
+
+end Lpofin
